coq/kernel/ConeDerivation.v
@@ -1,0 +1,29 @@
+From Coq Require Import List.
+From Coq Require Import FunctionalExtensionality.
+
+From Kernel Require Import VMStep KernelPhysics.
+
+Import ListNotations.
+
+Definition cone_like (f : list vm_instruction -> list nat) : Prop :=
+  f [] = [] /\
+  (forall i rest, f (i :: rest) = instr_targets i ++ f rest).
+
+Theorem Cone_Structure_Unique :
+  forall f,
+    cone_like f ->
+    forall trace, f trace = causal_cone trace.
+Proof.
+  intros f [Hnil Hcons] trace.
+  induction trace as [|i rest IH].
+  - rewrite Hnil. reflexivity.
+  - rewrite Hcons. simpl. rewrite IH. reflexivity.
+Qed.
+
+Theorem cone_monotone :
+  forall trace1 trace2 x,
+    In x (causal_cone trace1) -> In x (causal_cone (trace1 ++ trace2)).
+Proof.
+  intros trace1 trace2 x Hin.
+  eapply cone_monotonic; eauto.
+Qed.
